## explanation of the g() function.

This file attempts to explain the g() function. Or atleast how I arrived at developing it.

given that:
f(2n) = n/2
f(2n+1) = 3n+1

we can see that the pattern translates to a pattern of 4x+(0,1,2,3) such that:
(4x+0)/2 = 2n    (potentially 4x+2 or 4x+0)
(4x+1)   = 2n+1
(4x+2)/2 = 2n+1
(4x+3)   = 2n+1

so that (4x+2)/2 translates to (4x+{1,3})

2/2 = 1   (4x+1) ; 3\*1+1  = 4  (4x)
6/2 = 3   (4x+3) ; 3\*3+1  = 10 (4x+2)
10/2 = 5  (4x+1) ; 3\*5+1  = 16 (4x)
14/2 = 7  (4x+3) ; 3\*7+1  = 22 (4x+2)
18/2 = 9  (4x+1) ; 3\*9+1  = 28 (4x)
22/2 = 11 (4x+3) ; 3\*11+1 = 34 (4x+2)
26/2 = 13 (4x+1) ; 3\*13+1 = 40 (4x)
30/2 = 15 (4x+3) ; 3\*15+1 = 46 (4x+2)

as you can see from above 4x+{1,3} translates to 4x+{0,2}
so that we can say:

f(4x+1) -> f(4x+0)
f(4x+3) -> f(4x+2)

however, 4x+2 does not always go to 4x+1, it could go to 4x+3, how do we know? well:

f(4\*1+3) -> f(4\*5+2) -> f(4\*2+3)  -> f(4\*8+2)
f(4\*8+2) -> f(4\*4+1) -> f(4\*13+0) -> f(4\*6+2)
f(4\*6+2) -> f(4\*3+1) -> f(4\*10+0) -> f(4\*5+0)
f(4\*5+0) -> f(4\*2+2) -> f(4\*1+1)  -> f(4\*4+0)
f(4\*4+0) -> f(4\*2+0) -> f(4\*1+0)  -> f(4\*0+2)
f(4\*0+2) -> f(4\*0+1) -> f(4\*1+0)  -> f(4\*0+2)

f(4x+2) -> f(4y+3)  (x is odd)
f(4x+2) -> f(4y+1)  (x is even)

f(4\*7+2) -> f(4x+3) ? : 30 / 2 -> 15 (4\*3+3)
f(4\*20+2) -> f(4x+1)? : 82 / 2 -> 41 (4\*10+1)
f(4\*11+2) -> f(4\*5+3) : f(46) -> f(23)
f(4\*18+2) -> f(4\*9+1) : f(74) -> f(37)

if x is odd, transform 4x+2 to 4y+3  (move up)
if x is even, transform 4x+2 to 4y+1 (move down)

4x+1 always moves to 4y+0
4x+3 always moves to 4y+2
where y is floor(x/2)

f(4\*0+2)  -> f(4\*0+1) : f(2)  -> f(1)
f(4\*1+2)  -> f(4\*0+3) : f(6)  -> f(3)
f(4\*2+2)  -> f(4\*1+1) : f(10) -> f(5)
f(4\*3+2)  -> f(4\*1+3) : f(14) -> f(7)
f(4\*4+2)  -> f(4\*2+1) : f(18) -> f(9)
f(4\*5+2)  -> f(4\*2+3) : f(22) -> f(11)

we can see that
4x+2 -> 4y+3 when (x & 1)
4x+2 -> 4y+1 when !(x & 1)
4x+2 -> 4y+z ->
         y = floor(x/2)
	 z = 2 + -1^(x+1)

ok, so that explains 4x+2's pattern of transformation, how does 4x+1 transform x into y?
When we look at the following table what do we notice?

f(4\*0+1) -> f(4\*1+0)  : f(1)  -> f(4)
f(4\*1+1) -> f(4\*4+0)  : f(5)  -> f(16)
f(4\*2+1) -> f(4\*7+0)  : f(9)  -> f(28)
f(4\*3+1) -> f(4\*10+0) : f(13) -> f(40)
f(4\*4+1) -> f(4\*13+0) : f(17) -> f(52)
f(4\*5+1) -> f(4\*16+0) : f(21) -> f(64)
f(4\*6+1) -> f(4\*19+0) : f(25) -> f(76)
f(4\*7+1) -> f(4\*22+0) : f(29) -> f(88)

Upon inspection we can see that given a number of the form 4x+1 will result in a number whose form is 4y+0 where y = 3x+1, so:
f(4x+1) -> 4 \* (3 \* x + 1)

f(4\*22+1) -> 4 \* (3 \* 22 + 1) = 4 \* 67 = 268
f(89)      -> f(268)

f(4\*101+1) -> 4 \* (3 \* 101 + 1) = 4 \* 304 = 1216
f(405)     -> f(1216)

Now that we've figured out the pattern of transformation for numbers of the form 4x+1, the only number remaining is
numbers of the form 4x+3. Here's another table to help us out:

f(4\*0+3) -> f(4\*2+2)  : f(3)  -> f(10)
f(4\*1+3) -> f(4\*5+2)  : f(7)  -> f(22)
f(4\*2+3) -> f(4\*8+2)  : f(11) -> f(34)
f(4\*3+3) -> f(4\*11+2) : f(15) -> f(46)
f(4\*4+3) -> f(4\*14+2) : f(19) -> f(58)

We can see, that much like 4x+1, 4x+3 uses a similar formula, the only difference? instead of y=3n+1, we have y=3n+2
f(4x+3) -> 4 \* (3 \* x + 2) + 2

f(4\*22+3) -> 4 \* (3 \* 22 + 2) + 2 = 4 \* 68 + 2 = 274
f(91)     -> f(274)

f(4\*43+3) -> 4 \* (3 \* 43 + 2) + 2 = 4 \* 131 + 2 = 526
f(175)    -> f(526)

Lets recap, originally we defined the function as follows:
f(2n)   -> n/2
f(2n+1) -> 3n+1

but with our new found knowledge we can define it further as:
f(4n+0)   -> n/2
f(4n+1)   -> 4 \* (3 \* (n/4) + 1)
f(4n+2)   -> 4 \* floor(n/8) + (2 + -1^((n/4)+1))
f(4n+3)   -> 4 \* (3 \* (n/4) + 2) + 2

By following this function through we can see that:

f(4x+1) will always generate a number that is of the form 4x+0
f(4x+3) will always generate a number that is of the form 4x+2
f(4x+2) will split based on whether or not a given x is odd or even
f(4x+0) will always result in halving the number, this could lead back to forms of 4x+{0,1,2,3}
